AP/Dir.lean
@@ -9,17 +9,56 @@ deriving Inhabited, DecidableEq, Fintype
 
 namespace Dir
 
-def point : Dir → PointZ
-| .up => ⟨0, -1⟩
-| .down => ⟨0, 1⟩
-| .left => ⟨-1, 0⟩
-| .right => ⟨1, 0⟩
+open Dir
 
-@[simp] theorem point_up : Dir.up.point = ⟨0, -1⟩ := rfl
-@[simp] theorem point_down : Dir.down.point = ⟨0, 1⟩ := rfl
-@[simp] theorem point_left : Dir.left.point = ⟨-1, 0⟩ := rfl
-@[simp] theorem point_right : Dir.right.point = ⟨1, 0⟩ := rfl
+def point : Dir → PointZ
+| up => ⟨0, -1⟩
+| down => ⟨0, 1⟩
+| left => ⟨-1, 0⟩
+| right => ⟨1, 0⟩
+
+@[simp] theorem point_up : up.point = ⟨0, -1⟩ := rfl
+@[simp] theorem point_down : down.point = ⟨0, 1⟩ := rfl
+@[simp] theorem point_left : left.point = ⟨-1, 0⟩ := rfl
+@[simp] theorem point_right : right.point = ⟨1, 0⟩ := rfl
 
 @[simp]
 theorem point_ne_zero {t : Dir} : t.point ≠ 0 := by
   cases t <;> decide
+
+def hor : Dir → Prop
+| left => True
+| right => True
+| _ => False
+
+def vert : Dir → Prop
+| up => True
+| down => True
+| _ => False
+
+@[simp] theorem not_hor_up : ¬up.hor := λ h => h
+@[simp] theorem not_hor_down : ¬down.hor := λ h => h
+@[simp] theorem hor_left : left.hor := trivial
+@[simp] theorem hor_right : right.hor := trivial
+
+@[simp] theorem vert_up : up.vert := trivial
+@[simp] theorem vert_down : down.vert := trivial
+@[simp] theorem not_vert_left : ¬left.vert := λ h => h
+@[simp] theorem not_vert_right : ¬right.vert := λ h => h
+
+@[simp] theorem not_hor {d : Dir} : ¬d.hor ↔ d.vert := by cases d <;> simp
+@[simp] theorem not_vert {d : Dir} : ¬d.vert ↔ d.hor := by cases d <;> simp
+
+instance {d : Dir} : Decidable d.hor :=
+  match d with
+  | up => .isFalse # λ h => h
+  | down => .isFalse # λ h => h
+  | left => .isTrue trivial
+  | right => .isTrue trivial
+
+instance {d : Dir} : Decidable d.vert :=
+  match d with
+  | up => .isTrue trivial
+  | down => .isTrue trivial
+  | left => .isFalse # λ h => h
+  | right => .isFalse # λ h => h
